\begin{multline*}
f=\widebar{x_1}\widebar{x_2} \cdot f(00 x_3 x_4) \lor \widebar{x_1}x_2 \cdot f(01 x_3 x_4) \lor x_1\widebar{x_2} \cdot f(10 x_3 x_4) \lor x_1x_2 \cdot f(11 x_3 x_4)=\\
=\widebar{x_1}\widebar{x_2} \cdot (\widebar{0} \cdot \widebar{0} \cdot x_3 \lor 0 \cdot x_3\widebar{x_4} \lor \widebar{0} \cdot \widebar{x_3}x_4) \lor \\ \lor \widebar{x_1}x_2(\widebar{0} \cdot \widebar{1} \cdot x_3 \lor 0 \cdot x_3\widebar{x_4} \lor \widebar{1} \cdot \widebar{x_3}x_4) \lor \\ \lor x_1\widebar{x_2}(\widebar{1} \cdot \widebar{0} \cdot x_3 \lor 1 \cdot x_3\widebar{x_4} \lor \widebar{0} \cdot \widebar{x_3}x_4) \lor \\ \lor x_1x_2(\widebar{1}\widebar{1} \cdot x_3 \lor 1 \cdot x_3\widebar{x_4} \lor \widebar{1} \cdot \widebar{x_3}x_4)=\\
=\widebar{x_1}\widebar{x_2}(x_3 \lor \widebar{x_3}x_4) \lor \widebar{x_1}x_2 \cdot 0 \lor x_1\widebar{x_2}(x_3\widebar{x_4} \lor \widebar{x_3}x_4) \lor x_1x_2(x_3\widebar{x_4})=\\
=\widebar{x_1}\widebar{x_2}(x_3 \lor \cancel{\widebar{x_3}}x_4) \lor x_1\widebar{x_2}(x_3\widebar{x_4} \lor \widebar{x_3}x_4) \lor x_1x_2(x_3\widebar{x_4})\\
\end{multline*}